# MCR3U Final Examination – Answer Key (Jan 2023)

This key corresponds to `final-exam-2023.md`. Exact values are used where appropriate; approximations are indicated.

---

## Part A – Short Answers

1. **If** $f(x) = -2\sqrt{2x-1} + 5$, **determine** $f(5)$.

   $2(5) - 1 = 9$, $\sqrt{9} = 3$  \\
   $f(5) = -2(3) + 5 = -6 + 5 = \boxed{-1}$

2. For $y = -2(x+3)^2 + 7$:

   - (a) **Vertex**: already in vertex form $a(x-h)^2 + k$ with $h=-3, k=7$  \\
     $\Rightarrow \boxed{(-3, 7)}$
   - (b) **$y$-intercept**: set $x=0$  \\
     $y = -2(3)^2 + 7 = -18 + 7 = -11$  \\
     $\Rightarrow \boxed{(0, -11)}$
   - (c) **Max value**: opens down ($a=-2<0$), so max is $y$-value of vertex  \\
     $\Rightarrow \boxed{7}$
   - (d) **Domain**: parabola defined for all real $x$  \\
     $\Rightarrow \boxed{\mathbb{R}}$
   - (e) **Range**: $y$ is at most $7$  \\
     $\Rightarrow \boxed{y \le 7}$

3. For $y = \dfrac{3}{x-1} + 2$:

   - (a) **Parent function**: $\boxed{y = \dfrac{1}{x}}$
   - (b) **Vertical stretch factor**: coefficient of parent is $3$  \\
     $\Rightarrow \boxed{3}$
   - (c) **Horizontal translation**: $x-1$ in denominator means 1 unit right  \\
     $\Rightarrow \boxed{1\text{ unit right}}$

4. **State the inverse of:**

   - (a) $f(x) = x - 3$  \\
     $y = x-3 \Rightarrow x = y-3 \Rightarrow y = x+3$  \\
     $\boxed{f^{-1}(x) = x+3}$
   - (b) $f(x) = 3x$  \\
     $y = 3x \Rightarrow x = 3y \Rightarrow y = \dfrac{x}{3}$  \\
     $\boxed{f^{-1}(x) = \dfrac{x}{3}}$
   - (c) $f(x) = x^2$  \\
     Inverse relation: $y = \pm\sqrt{x}$; as a function, with domain restricted to $x\ge0$, $\boxed{f^{-1}(x) = \sqrt{x}}$.

5. **Simplify:**

   - (a) $\dfrac{3x}{5x} = \dfrac{3}{5}$ (for $x\ne 0$)  \\
     $\Rightarrow \boxed{\dfrac{3}{5}}$
   - (b) $\dfrac{x(x-3)^2}{x^2(x-3)} = \dfrac{(x-3)}{x}$ (cancel one $x$ and one $(x-3)$)  \\
     $\Rightarrow \boxed{\dfrac{x-3}{x}}$

6. **Factor:**

   - (a) $5m^2 - 25m = 5m(m-5)$  \\
     $\boxed{5m(m-5)}$
   - (b) $m^2 - 4m - 5 = (m-5)(m+1)$  \\
     $\boxed{(m-5)(m+1)}$
   - (c) $2x^2 + 3x - 9 = (2x-3)(x+3)$  \\
     $\boxed{(2x-3)(x+3)}$

7. For $f(x) = -2x^2 - 8x$:

   - (a) **$y$-intercept**: $f(0) = 0$  \\
     $\boxed{(0, 0)}$
   - (b) **Direction of opening**: $a = -2 < 0$  \\
     $\boxed{\text{downward}}$
   - (c) **Zeros**: $-2x^2 - 8x = -2x(x+4) = 0 \Rightarrow x=0,-4$  \\
     $\boxed{(0,0),\ (-4,0)}$
   - (d) **Vertex**: midpoint of zeros is $x=-2$; $f(-2) = 8$  \\
     $\boxed{(-2, 8)}$

8. **Reduce** $\sqrt{12}$:

   $\sqrt{12} = \sqrt{4\cdot3} = 2\sqrt{3} \Rightarrow \boxed{2\sqrt{3}}$

9. **Exact value of** $\cos 60^\circ$:

   $\boxed{\dfrac{1}{2}}$

10. **Related acute angle for** $300^\circ$:

    $360^\circ - 300^\circ = 60^\circ \Rightarrow \boxed{60^\circ}$

11. **Point** $P(-5,-6)$ on terminal arm

    $x=-5,\ y=-6,\ r = \sqrt{(-5)^2 + (-6)^2} = \sqrt{61}$.

    - (a) $\cot\theta = \dfrac{\cos\theta}{\sin\theta} = \dfrac{x/r}{y/r} = \dfrac{x}{y} = \dfrac{-5}{-6} = \boxed{\dfrac{5}{6}}$
    - (b) Related acute angle: $\tan\alpha = \left|\dfrac{y}{x}\right| = \dfrac{6}{5}$  \\
      $\Rightarrow \alpha \approx \tan^{-1}\left(\dfrac{6}{5}\right) \approx \boxed{50.2^\circ}$ (1 d.p.)
    - (c) Quadrant III, so $\theta = 180^\circ + \alpha \approx 180^\circ + 50.2^\circ = \boxed{230.2^\circ}$ (1 d.p.)

12. For $y = -3\cos(10(x+9)) + 2$:

    - (a) **Phase shift**: $x+9 = x-(-9)$  \\
      $\Rightarrow$ shift $\boxed{9\ \text{units left}}$
    - (b) **Amplitude**: $\boxed{3}$
    - (c) **Period**: $T = \dfrac{2\pi}{|10|} = \boxed{\dfrac{\pi}{5}}$
    - (d) **Axis (midline)**: $\boxed{y = 2}$
    - (e) **Max value**: $2 + 3 = \boxed{5}$
    - (f) **Min value**: $2 - 3 = \boxed{-1}$

13. **Simplify with positive exponents:**

    - (a) $\dfrac{3x^2}{27x} = \dfrac{3}{27}\cdot\dfrac{x^2}{x} = \dfrac{1}{9}x = \boxed{\dfrac{x}{9}}$
    - (b) $\dfrac{(4x)^2}{2x^6} = \dfrac{16x^2}{2x^6} = \dfrac{8}{x^4}$  \\
      $\boxed{\dfrac{8}{x^4}}$
    - (c) $\left(\dfrac{3x^{-1}}{x^3}\right)^{-2} = (3x^{-4})^{-2} = 3^{-2}x^8 = \boxed{\dfrac{x^8}{9}}$
    - (d) $\dfrac{\sqrt[3]{x^4}}{\sqrt{x}} = \dfrac{x^{4/3}}{x^{1/2}} = x^{5/6}$  \\
      $\boxed{x^{5/6}}$

---

## Part B – Full Solutions

1. **Simplify** $\dfrac{m^{2}-4m-5}{5m^{2}-25m} \div \dfrac{m^{2}+3m+2}{15m^{2}}$.

   Factor:

   - $m^{2}-4m-5 = (m-5)(m+1)$
   - $5m^{2}-25m = 5m(m-5)$
   - $m^{2}+3m+2 = (m+1)(m+2)$

  $\frac{(m-5)(m+1)}{5m(m-5)} \div \frac{(m+1)(m+2)}{15m^{2}}$
  $= \frac{m+1}{5m} \times \frac{15m^{2}}{(m+1)(m+2)}$

   Cancel $(m+1)$ and one $m$; $15/5 = 3$:

  $= \frac{3m}{m+2}$

   So $\boxed{\dfrac{3m}{m+2}}$ (restrictions: $m\ne 0,-2,5,-1$).

---

2. **Solve the quadratic equations.**

   (a) $2x^{2} - 9x - 5 = 0$

   Factor by grouping:

  $2x^{2} - 9x - 5 = 2x^{2} - 10x + x - 5$
  $= 2x(x-5) + 1(x-5) = (2x+1)(x-5)$

   Set each factor to zero:

  $2x+1=0 \Rightarrow x=-\frac{1}{2}, \quad x-5=0 \Rightarrow x=5$

   So $\boxed{x = -\dfrac{1}{2},\ 5}$.

   ---

   (b) $2x^{2} + 2.7x - 5.1 = 0$

   Use the quadratic formula, $a=2, b=2.7, c=-5.1$:

  $$x = \frac{-b \pm \sqrt{b^{2} - 4ac}}{2a} = \frac{-2.7 \pm \sqrt{2.7^{2} - 4(2)(-5.1)}}{4}$$

  $$b^{2} - 4ac = 7.29 + 40.8 = 48.09$$

  $$x = \frac{-2.7 \pm \sqrt{48.09}}{4}$$

   $\sqrt{48.09} \approx 6.93$:

  $x_1 \approx \frac{-2.7 + 6.93}{4} \approx 1.06, \quad$
  $x_2 \approx \frac{-2.7 - 6.93}{4} \approx -2.41$

   So $\boxed{x \approx 1.06,\ -2.41}$ (to 2 decimal places).

---

3. **Simplify** $(7\sqrt{2} + \sqrt{3})(7\sqrt{2} - \sqrt{3})$.

   Recognize a difference of squares, $(a+b)(a-b) = a^{2} - b^{2}$ with $a=7\sqrt{2}$, $b=\sqrt{3}$:

  $(7\sqrt{2})^{2} - (\sqrt{3})^{2} = 49\cdot 2 - 3 = 98 - 3 = 95$

   So $\boxed{95}$.

---

4. **Projectile problem** – $h(t) = -5t^{2} + 20t + 0.8$

   (a) **Initial height** (when the ball is hit): set $t=0$.

  $h(0) = -5(0)^{2} + 20(0) + 0.8 = 0.8$

   So the ball is $\boxed{0.8\ \text{m}}$ above the ground when hit.

   ---

   (b) **Maximum height**: vertex of the parabola.

   For $h(t) = at^{2} + bt + c$ with $a=-5, b=20$:

  $t_{\text{max}} = -\frac{b}{2a} = -\frac{20}{2(-5)} = 2\ \text{s}$

  $h(2) = -5(2)^{2} + 20(2) + 0.8 = -20 + 40 + 0.8 = 20.8$

   So the maximum height is $\boxed{20.8\ \text{m}}$.

   ---

   (c) **Time when the ball hits the ground**: solve $h(t)=0$.

  $-5t^{2} + 20t + 0.8 = 0$

   Quadratic formula with $a=-5, b=20, c=0.8$:

  $t = \frac{-20 \pm \sqrt{20^{2} - 4(-5)(0.8)}}{2(-5)}$
  $= \frac{-20 \pm \sqrt{400 + 16}}{-10}$
  $= \frac{-20 \pm \sqrt{416}}{-10}$

   $\sqrt{416} \approx 20.4$ gives one negative and one positive root; the physical solution is the positive time:

  $t \approx 4.04\ \text{s}$

   So the ball hits the ground at about $\boxed{4.0\ \text{s}}$ (to 1 d.p.).

---

5. **Diagram problem (length $x$)**

   Using labels: bottom left $A$, middle bottom $B$, bottom right $C$, top point $D$.

   Given:

   - $AD = 37\,\text{m}$
   - $\angle DAB = 100^\circ$
   - $\angle D = 22^\circ$ (between $AD$ and $DB$)
   - $BC = 25\,\text{m}$
   - Need $DC = x$.

   **Step 1: Triangle $\triangle DAB$**

   Angles in triangle:

  $\angle DAB = 100^\circ,\ \angle D = 22^\circ$
  $\Rightarrow \angle B = 180^\circ - 100^\circ - 22^\circ = 58^\circ$

   Apply the sine law:

  $\frac{AD}{\sin \angle B} = \frac{AB}{\sin \angle D}$
  $\Rightarrow$
  $\frac{37}{\sin 58^\circ} = \frac{AB}{\sin 22^\circ}$

  $AB = 37 \cdot \frac{\sin 22^\circ}{\sin 58^\circ} \approx 16.3\,\text{m}$

   So

  $AC = AB + BC \approx 16.3 + 25 = 41.3\,\text{m}.$

   **Step 2: Triangle $\triangle DAC$**

   Now $AD = 37$, $AC \approx 41.3$, and the included angle at $A$ is still $100^\circ$.

   Apply the cosine law:

  $DC^{2} = AD^{2} + AC^{2} - 2(AD)(AC)\cos 100^\circ$

  $DC^{2} \approx 37^{2} + 41.3^{2} - 2(37)(41.3)\cos 100^\circ \approx 3609$

  $DC \approx \sqrt{3609} \approx 60.1\,\text{m}$

   So $\boxed{x \approx 60.1\,\text{m}}$ (to one decimal place).

---

6. **For** $\cos(A) = -\dfrac{2}{3}$, $0^\circ \le A \le 360^\circ$.

   (a) **Sketch**: cosine negative in quadrants II and III, so terminal arms lie in QII and QIII.

   (b) **Exact values of** $\tan(A)$

  $\cos^2 A = \left(-\frac{2}{3}\right)^2 = \frac{4}{9},\ \sin^2 A = 1 - \frac{4}{9} = \frac{5}{9}$

   So $|\sin A| = \dfrac{\sqrt{5}}{3}$.

   - In QII: $\sin A = \dfrac{\sqrt{5}}{3}$, $\cos A = -\dfrac{2}{3}$  \\
     $\displaystyle \tan A = \frac{\sin A}{\cos A} = \frac{\sqrt{5}/3}{-2/3} = -\frac{\sqrt{5}}{2}$
   - In QIII: $\sin A = -\dfrac{\sqrt{5}}{3}$, $\cos A = -\dfrac{2}{3}$  \\
     $\displaystyle \tan A = \frac{-\sqrt{5}/3}{-2/3} = \frac{\sqrt{5}}{2}$

   So $\boxed{\tan A = -\dfrac{\sqrt{5}}{2}\ \text{(QII)},\ \tan A = \dfrac{\sqrt{5}}{2}\ \text{(QIII)}}$.

   ---

   (c) **Related acute angle and all values of $A$**

   Related acute angle:

  $\alpha = \cos^{-1}\left(\frac{2}{3}\right) \approx 48.2^\circ$

   Cosine is negative in quadrants II and III:

  $A_1 = 180^\circ - \alpha \approx 180^\circ - 48.2^\circ = 131.8^\circ$
  $A_2 = 180^\circ + \alpha \approx 180^\circ + 48.2^\circ = 228.2^\circ$

   So the related acute angle is $\boxed{48.2^\circ}$, and  \\
   $\boxed{A \approx 131.8^\circ,\ 228.2^\circ}$ (1 d.p.).

---

7. **Exponential transformation** – $y = 2 \cdot 3^{-2(x+1)} - 3$

   Let the parent be $f(x) = 3^{x}$.

   (a) **Pointwise formula and 3 key points**

   We can write the transformation as

  $y = 2 f(-2(x+1)) - 3.$

   Let $(x, y)$ lie on $y = 3^{x}$ (so $y = 3^{x}$). For the image point $(X, Y)$:

  $x = -2(X+1) \Rightarrow X = -\frac{x}{2} - 1,\quad Y = 2y - 3.$

   So the pointwise rule is

  $\boxed{(x, y) \mapsto \left(-\frac{x}{2} - 1,\ 2y - 3\right)}.$

   Use three key points of $y=3^{x}$:

   - $(-1, \tfrac{1}{3}) \mapsto \left(-\tfrac{1}{2},\ -\tfrac{7}{3}\right)$
   - $(0, 1) \mapsto (-1, -1)$
   - $(1, 3) \mapsto \left(-\tfrac{3}{2},\ 3\right)$

   (b) **Graph of** $y = 2 \cdot 3^{-2(x+1)} - 3$

   Important features to label:

   - Horizontal asymptote as $x\to \infty$: $y \to -3$  \\
     $\Rightarrow$ asymptote $\boxed{y = -3}$
   - Example key points: $(-1, -1)$ and $\left(-\tfrac{3}{2}, 3\right)$ and $\left(-\tfrac{1}{2}, -\tfrac{7}{3}\right)$
   - $y$-intercept ($x=0$):  \\
     $y = 2\cdot3^{-2} - 3 = \dfrac{2}{9} - 3 = -\dfrac{25}{9}$.

   Plot these points and the asymptote to complete the sketch.

---

8. **Cosine transformation** – $y = -3\cos(10(x+9)) + 2$

   Parent: $y = \cos x$.

   (a) **Pointwise formula and 3 key points**

   Write

  $y = -3 f(10(x+9)) + 2,\quad \text{where } f(x) = \cos x.$

   If $(x, y)$ lies on $y=\cos x$, then for the image point $(X, Y)$:

  $x = 10(X+9) \Rightarrow X = \frac{x}{10} - 9,\quad Y = -3y + 2.$

   So

  $\boxed{(x, y) \mapsto \left(\frac{x}{10} - 9,\ -3y + 2\right)}.$

   Use three standard key points of $y=\cos x$ over $[0, 2\pi]$:

   - $(0, 1) \mapsto (-9, -1)$
   - $(\pi, -1) \mapsto \left(-9 + \tfrac{\pi}{10},\ 5\right)$
   - $(2\pi, 1) \mapsto \left(-9 + \tfrac{\pi}{5},\ -1\right)$

   (b) **Sketch one period of** $y = -3\cos(10(x+9)) + 2$

   Key characteristics:

   - Amplitude: $\boxed{3}$
   - Period: $T = \dfrac{2\pi}{10} = \boxed{\dfrac{\pi}{5}}$
   - Phase shift: $x+9 = x-(-9)$  \\
     $\Rightarrow$ shift $\boxed{9\ \text{units left}}$
   - Vertical shift / axis: $\boxed{y = 2}$
   - Max value: $2+3 = 5$; min value: $2-3 = -1$.

   Over one period from $x = -9$ to $x = -9 + \dfrac{\pi}{5}$, mark:

   - $(-9, -1)$ (minimum)
   - $\left(-9 + \dfrac{\pi}{10}, 5\right)$ (maximum)
   - $\left(-9 + \dfrac{\pi}{5}, -1\right)$ (minimum)

   Draw a cosine wave through these points around the axis $y=2$ to complete the sketch.
