
## 3U Ch.2 Test: Solution Key

### 1. Simplify the following

_State any restrictions (values that would make a denominator zero)._

-   **(a)**  $\frac{x}{x} = \mathbf{1}, \quad x \neq 0$ 1
    
-   **(b)**  $\frac{(x-3)^{2}}{x-3} = \mathbf{x-3}, \quad x \neq 3$ 2
    
-   **(c)**  $\frac{x+7}{(x+7)^{2}} = \mathbf{\frac{1}{x+7}}, \quad x \neq -7$ 3
    
-   **(d)**  $\frac{x^{2}y^{3}}{yx^{3}} = \mathbf{\frac{y^{2}}{x}}, \quad x \neq 0, y \neq 0$ 4
    
-   **(e)**  $\frac{1}{x} \div \frac{1}{y} = \frac{1}{x} \times \frac{y}{1} = \mathbf{\frac{y}{x}}, \quad x \neq 0, y \neq 0$ 5
    
-   **(f)**  $\frac{(3x-5)^{2}(x+1)}{(x+1)^{2}(3x-5)} = \mathbf{\frac{3x-5}{x+1}}, \quad x \neq -1, \frac{5}{3}$ 6
    

----------

### 2. Factor

_These are the building blocks for simplifying rational expressions._

-   **(a)**  $5m^{2}-25m = \mathbf{5m(m-5)}$ 7
    
-   **(b)**  $m^{2}-4m-5 = \mathbf{(m-5)(m+1)}$ 8
    
-   **(c)**  $m^{2}+3m+2 = \mathbf{(m+2)(m+1)}$ 9
    
-   **(d)**  $x^{2}+3x-10 = \mathbf{(x+5)(x-2)}$ 10
    
-   **(e)**  $x^{2}-x-12 = \mathbf{(x-4)(x+3)}$ 11
    
-   **(f)**  $2x^{2}+5x+2 = \mathbf{(2x+1)(x+2)}$ 12
    
-   **(g)**  $x^{2}-2x-15 = \mathbf{(x-5)(x+3)}$ 13
    
-   **(h)**  $2x^{2}+x-6 = \mathbf{(2x-3)(x+2)}$ 14
    
-   **(i)**  $2x^{2}+7x+3 = \mathbf{(2x+1)(x+3)}$ 15
    
-   **(j)**  $2x^{2}+13x+15 = \mathbf{(2x+3)(x+5)}$ 16
    
-   **(k)**  $4x^{2}-9 = \mathbf{(2x-3)(2x+3)}$ 17
    
-   **(l)**  $3x^{2}-x-4 = \mathbf{(3x-4)(x+1)}$ 18
    
-   **(m)**  $9x^{2}-24x+16 = \mathbf{(3x-4)^{2}}$ 19
    

----------

### 3. Simplify

_Remember: Factor everything first, then cancel common factors in multiplication/division. For addition/subtraction, find a common denominator._

-   **(a)** $\frac{3m^{2}-12m-15}{5m^{3}-25m^{2}} \times \frac{15m^{2}}{6m^{2}+18m+12}$
    
    -   Factor: $\frac{3(m-5)(m+1)}{5m^2(m-5)} \times \frac{15m^2}{6(m+1)(m+2)}$ 20
        
    -   Cancel: $\frac{3}{1} \times \frac{3}{6(m+2)} = \frac{9}{6(m+2)} = \mathbf{\frac{3}{2(m+2)}}$
        
    -   **Restrictions:**  $m \neq 0, 5, -1, -2$ 21
        
-   **(b)** $\frac{5x+25}{x^{2}+3x-10} - \frac{4x-16}{x^{2}-x-12}$
    
    -   Simplify each fraction first: $\frac{5(x+5)}{(x+5)(x-2)} - \frac{4(x-4)}{(x-4)(x+3)}$ 22
        
    -   Result: $\frac{5}{x-2} - \frac{4}{x+3}$
        
    -   Common Denom: $\frac{5(x+3) - 4(x-2)}{(x-2)(x+3)} = \frac{5x+15-4x+8}{(x-2)(x+3)} = \mathbf{\frac{x+23}{(x-2)(x+3)}}$
        
    -   **Restrictions:**  $x \neq -5, 2, 4, -3$ 23
        
-   **(c)** $\frac{2x^{2}+5x+2}{2x^{2}+7x+3} \div \frac{2x^{2}+x-6}{x^{2}-2x-15}$
    
    -   Factor and Flip: $\frac{(2x+1)(x+2)}{(2x+1)(x+3)} \times \frac{(x-5)(x+3)}{(2x-3)(x+2)}$ 24
        
    -   Cancel: $\frac{1}{1} \times \frac{x-5}{2x-3} = \mathbf{\frac{x-5}{2x-3}}$
        
    -   **Restrictions:**  $x \neq -\frac{1}{2}, -3, \frac{3}{2}, -2, 5$ 25
        
-   **(d)** $\frac{2x^{2}+13x+15}{4x^{2}-9} + \frac{3x^{2}-x-4}{9x^{2}-24x+16}$
    
    -   Factor: $\frac{(2x+3)(x+5)}{(2x-3)(2x+3)} + \frac{(3x-4)(x+1)}{(3x-4)^2}$ 26
        
    -   Simplify: $\frac{x+5}{2x-3} + \frac{x+1}{3x-4}$
        
    -   Common Denom: $\frac{(x+5)(3x-4) + (x+1)(2x-3)}{(2x-3)(3x-4)}$
        
    -   Expand: $\frac{(3x^2+11x-20) + (2x^2-x-3)}{(2x-3)(3x-4)} = \mathbf{\frac{5x^2+10x-23}{(2x-3)(3x-4)}}$
        
    -   **Restrictions:**  $x \neq \pm \frac{3}{2}, \frac{4}{3}$ 27
