To graph or analyze the transformation of the function:

$$g(x) = 2(2)^{\frac{1}{3}(x+4)} + 1$$

You need to compare it to the standard transformation form: **$g(x) = a(b)^{k(x-d)} + c$**

Here is the step-by-step breakdown.

### 1. Identify the Parent Function
The base is **2**.
*   **Parent Function:** $f(x) = 2^x$
*   **Key Points on Parent:** $(-1, 0.5)$, $(0, 1)$, $(1, 2)$, $(2, 4)$
*   **Original Asymptote:** $y = 0$

---

### 2. Identify the Parameters ($a, k, d, c$)

**$a = 2$ (Vertical Stretch)**
*   Since $a > 1$, multiply all $y$-values by 2.
*   **Effect:** Vertical stretch by a factor of 2.

**$k = \frac{1}{3}$ (Horizontal Stretch)**
*   The horizontal factor is always the reciprocal $\frac{1}{k}$.
*   $\frac{1}{1/3} = 3$. Multiply all $x$-values by 3.
*   **Effect:** Horizontal stretch by a factor of 3.

**$d = -4$ (Horizontal Translation)**
*   Inside the bracket is $(x+4)$.
*   **Effect:** Shift Left 4 units.

**$c = 1$ (Vertical Translation)**
*   Added at the very end.
*   **Effect:** Shift Up 1 unit.

---

### 3. Use the Mapping Rule (The "Point Method")
This is the safest way to get your points correct for a graph.

**Formula:** $(x, y) \rightarrow (\frac{x}{k} + d, \quad ay + c)$

For your specific equation:
*   **x-values:** Multiply by 3, then subtract 4 ($3x - 4$).
*   **y-values:** Multiply by 2, then add 1 ($2y + 1$).

**Let's transform the key points:**

| Parent Point $(x, y)$ | Transform $x$ ($3x - 4$) | Transform $y$ ($2y + 1$) | **New Point** |
| :--- | :--- | :--- | :--- |
| **$(-1, 0.5)$** | $3(-1) - 4 = -7$ | $2(0.5) + 1 = 2$ | **$(-7, 2)$** |
| **$(0, 1)$** (y-int) | $3(0) - 4 = -4$ | $2(1) + 1 = 3$ | **$(-4, 3)$** |
| **$(1, 2)$** | $3(1) - 4 = -1$ | $2(2) + 1 = 5$ | **$(-1, 5)$** |
| **$(2, 4)$** | $3(2) - 4 = 2$ | $2(4) + 1 = 9$ | **$(2, 9)$** |

---

### 4. Summary of Final Features
If you are asked to list the properties of the new function $g(x)$:

*   **Equation of Asymptote:** The asymptote moves with the vertical shift ($c$).
    *   New Asymptote: **$y = 1$**
*   **Domain:** **$\{x \in \mathbb{R}\}$** (This never changes for exponential functions).
*   **Range:** Since $a$ is positive (graph goes up) and the asymptote is at 1:
    *   **$\{y \in \mathbb{R} \mid y > 1\}$**
*   **y-intercept:** To find the exact y-intercept, set $x=0$:
    *   $g(0) = 2(2)^{\frac{1}{3}(0+4)} + 1$
    *   $g(0) = 2(2)^{1.333} + 1 \approx 6.04$ (It's not a nice integer, so use the point $(-4, 3)$ as your reference point instead).